

Homework 6

1. $p(t) = x_0 + x_1 t + x_2 t^2$

$$\begin{array}{c|ccccc} t & -2 & -1 & 0 & 1 & 2 \\ \hline y & 2 & -10 & 0 & 2 & 1 \end{array}$$

let A be a 5×3 matrix and y be 5×1 vector

$$A = \begin{pmatrix} 1 & -2 & 4 \\ 1 & -1 & 1 \\ 1 & 0 & 0 \\ 1 & 1 & 1 \\ 1 & 2 & 4 \end{pmatrix} \quad y = \begin{pmatrix} 2 \\ -10 \\ 0 \\ 2 \\ 1 \end{pmatrix}$$

$$A^T A = \begin{pmatrix} 1 & 1 & 1 & 1 & 1 \\ -2 & -1 & 0 & 1 & 2 \\ 4 & 1 & 0 & 1 & 4 \end{pmatrix} \begin{pmatrix} 1 & -2 & 4 \\ 1 & -1 & 1 \\ 1 & 0 & 0 \\ 1 & 1 & 1 \\ 1 & 2 & 4 \end{pmatrix} = \begin{pmatrix} 5 & 0 & 10 \\ 0 & 10 & 0 \\ 10 & 0 & 34 \end{pmatrix}$$

$$A^T y = \begin{pmatrix} 1 & 1 & 1 & 1 & 1 \\ -2 & -1 & 0 & 1 & 2 \\ 4 & 1 & 0 & 1 & 4 \end{pmatrix} \begin{pmatrix} 2 \\ -10 \\ 0 \\ 2 \\ 1 \end{pmatrix} = \begin{pmatrix} -5 \\ 10 \\ 4 \end{pmatrix}$$

$$\det(A^T A) = 5 \times 10 \times 34 + 0 + 0 - 10 \times 10 \times 10 - 0 - 0 = 700$$

$$M_{11} = 10 \times 34 - 0 = 340; \quad M_{12} = -(0 - 0) = 0; \quad M_{13} = 0 - 10 \times 10 = -100$$

$$M_{21} = -(0 - 0) = 0; \quad M_{22} = 5 \times 34 - 10 \times 10 = 70; \quad M_{23} = -(0 - 0) = 0$$

$$M_{31} = 0 - 10 \times 10 = -100; \quad M_{32} = -(0 - 0) = 0; \quad M_{33} = 5 \times 10 - 0 = 50$$

$$(A^T A)^{-1} = \frac{1}{\det(A^T A)} \text{adj}(A^T A) = \frac{1}{700} \begin{pmatrix} 340 & 0 & -100 \\ 0 & 70 & 0 \\ -100 & 0 & 50 \end{pmatrix}$$

Thus, $A^T A x = A^T y$

$$\begin{aligned} x &= (A^T A)^{-1} A^T y = \frac{1}{700} \begin{pmatrix} 340 & 0 & -100 \\ 0 & 70 & 0 \\ -100 & 0 & 50 \end{pmatrix} \begin{pmatrix} -5 \\ 10 \\ 4 \end{pmatrix} \\ &= \frac{1}{700} \begin{pmatrix} -2100 \\ 700 \\ 700 \end{pmatrix} = \begin{pmatrix} -3 \\ 1 \\ 1 \end{pmatrix} \end{aligned}$$

Therefore, $p(t) = -3 + t + t^2$

2. $\begin{pmatrix} I & A \\ A^T & 0 \end{pmatrix} \begin{pmatrix} r \\ x \end{pmatrix} = \begin{pmatrix} b \\ 0 \end{pmatrix}$

$$\Rightarrow \begin{cases} I r + A x = b \\ A^T r + 0 \cdot x = 0 \end{cases} \Rightarrow \begin{cases} I r = b - A x \\ A^T r = 0 \end{cases}$$

Since $r = b - Ax$, we have $A^T(b - Ax) = 0$

$A^T A x = A^T b$. This is the solution to the least squares optimization problem of $\min \|Ax - b\|^2$

Therefore, $\min \|Ax - b\|^2$ can be obtained from solving $\begin{pmatrix} I & A \\ A^T & 0 \end{pmatrix} \begin{pmatrix} x \\ r \end{pmatrix} = \begin{pmatrix} b \\ 0 \end{pmatrix}$

3. $f(x) = \frac{1}{2} x^T Q x - c^T x$

(a) $\nabla f(x) = \frac{\partial}{\partial x} \left(\frac{1}{2} x^T Q x - c^T x \right) = Qx - c$

$Hf(x) = Q^T = Q$

(b) $f(x) \approx f(a) + \nabla f(a)^T (x - a) + \frac{1}{2} (x - a)^T \nabla^2 f(a) (x - a)$
 $\approx \frac{1}{2} a^T Q a - c^T a + (Qa - c)^T (x - a) + \frac{1}{2} (x - a)^T Q (x - a)$

(c) Since r^* is the optimal step size, we have $r^* = \operatorname{argmin}_r f(x - r \nabla f(x))$

$$\begin{aligned} f(x - r \nabla f(x)) &= \frac{1}{2} (x - r \nabla f(x))^T Q (x - r \nabla f(x)) - c^T (x - r \nabla f(x)) \\ &= \frac{1}{2} (x^T Q x - r \nabla f(x)^T Q x - r \nabla f(x)^T Q x + r^2 \nabla f(x)^T Q \nabla f(x)) - c^T x + r c^T \nabla f(x) \\ &= \left(\frac{1}{2} x^T Q x - c^T x \right) + \frac{1}{2} r^2 \nabla f(x)^T Q \nabla f(x) - r x^T Q \nabla f(x) + r c^T \nabla f(x) \\ &= f(x) + \frac{1}{2} r^2 (Qx - c)^T Q (Qx - c) - r (x^T Q (Qx - c) + c^T (Qx - c)) \end{aligned}$$

$$\begin{aligned} \frac{\partial}{\partial r} f(x - r \nabla f(x)) &= r (Qx - c)^T Q (Qx - c) - (x^T Q Qx - x^T Q c + c^T Qx - c^T c) = 0 \\ \Rightarrow r^* &= \frac{x^T Q Qx - c^T c}{(Qx - c)^T Q (Qx - c)} = \frac{(Qx - c)^T (Qx - c)}{(Qx - c)^T Q (Qx - c)} \end{aligned}$$

non zero vectors

4. Suppose $d_1, \dots, d_n \in \mathbb{R}^n$ are not linearly independent, then

$\exists \alpha_1, \dots, \alpha_n$ not all zero, such that $\alpha_1 d_1 + \alpha_2 d_2 + \dots + \alpha_n d_n = \sum_{j=1}^n \alpha_j d_j = 0$

Thus, we have $d_i^T Q \left(\sum_{j=1}^n \alpha_j d_j \right) = 0$

Since $d_i^T Q d_j = 0$ for all i, j with $i \neq j$, we can get

$$\sum_{j=1}^n \alpha_j d_i^T Q d_j = \alpha_i d_i^T Q d_i = 0$$

Because Q is a $n \times n$ symmetric and positive definite matrix

$$x^T Q x > 0, \forall x \in \mathbb{R}^n, \quad d_i^T Q d_i > 0$$

This means $\alpha_i = 0$ for each i

This result contradicts the assumption that $\alpha_1, \dots, \alpha_n$ are not all zero

Therefore, d_1, \dots, d_n are linearly independent in the standard sense

$$5. (a) \quad x^* - x^0 = \alpha_0 d_0 + \dots + \alpha_{n-1} d_{n-1} = \sum_{i=0}^{n-1} \alpha_i d_i$$

$$d_k^T Q (x^* - x^0) = \alpha_0 d_k^T Q d_0 + \dots + \alpha_{n-1} d_k^T Q d_{n-1}$$

Since $d_i^T Q d_j = 0$ for $i \neq j$, then we have

$$d_k^T Q (x^* - x^0) = \alpha_k d_k^T Q d_k$$

$$\text{Thus, } \alpha_k = \frac{d_k^T Q (x^* - x^0)}{d_k^T Q d_k}$$

$$(b) \quad x^{k+1} = x^k + \alpha_k d_k \Rightarrow x^k = x^0 + \alpha_0 d_0 + \dots + \alpha_{k-1} d_{k-1}$$

$$\text{Substituting } k=n, \text{ we have } x^n = x^0 + \alpha_0 d_0 + \dots + \alpha_{n-1} d_{n-1}$$

$$\text{Since } x^* - x_0 = \sum_{i=0}^{n-1} \alpha_i d_i \quad = x^0 + \sum_{i=0}^{n-1} \alpha_i d_i$$

it follows that $x^* = x^n$

For $x^k = x^0 + \sum_{i=0}^{k-1} \alpha_i d_i$, apply $d_k^T Q$

$$d_k^T Q x^k = d_k^T Q x^0 + d_k^T Q \sum_{i=0}^{k-1} \alpha_i d_i$$

$$= d_k^T Q x^0 + \alpha_0 d_k^T Q d_0 + \dots + \alpha_{k-1} d_k^T Q d_{k-1}$$

$$= d_k^T Q x^0$$

$$\text{Thus, } d_k^T Q x^k = d_k^T Q x^0$$

$$(c) \quad d_k^T Q x^0 = d_k^T Q x^k$$

$$d_k^T Q (x^* - x^0) = d_k^T Q (x^* - x^k)$$

$$= d_k^T (Ax^* - Ax^k)$$

$$= d_k^T (b - Ax^k) \quad \text{since } g_k = Ax^k - b$$

$$= d_k^T (-g_k) = -d_k^T g_k = -g_k^T d_k$$

$$\text{Thus, } d_k^T A(x^* - x^0) = -g_k^T d_k$$

$$\text{Since } \alpha_k = \frac{d_k^T A(x^* - x^0)}{d_k^T A d_k} \quad \text{obtained in part (a)}$$

$$\text{we can get } \alpha_k = \frac{-g_k^T d_k}{d_k^T A d_k}$$

$$6. (a) \quad A = \begin{pmatrix} 1 & 1 & 1 \\ 0 & 1 & 1 \\ 0 & 0 & 1 \end{pmatrix}, \quad d_0 = \begin{pmatrix} 1 \\ 0 \\ 0 \end{pmatrix}, \quad d_1 = \begin{pmatrix} 1 \\ 0 \\ -1 \end{pmatrix}, \quad d_2 = \begin{pmatrix} 1 \\ -1 \\ 0 \end{pmatrix}$$

$$d_0^T A d_1 = (1 \ 0 \ 0) \begin{pmatrix} 1 & 1 & 1 \\ 0 & 1 & 1 \\ 0 & 0 & 1 \end{pmatrix} \begin{pmatrix} 1 \\ 0 \\ -1 \end{pmatrix} = (1 \ 1 \ 1) \begin{pmatrix} 1 \\ 0 \\ -1 \end{pmatrix} = 0$$

$$d_0^T A d_2 = (1 \ 0 \ 0) \begin{pmatrix} 1 & 1 & 1 \\ 0 & 1 & 1 \\ 0 & 0 & 1 \end{pmatrix} \begin{pmatrix} 1 \\ -1 \\ 0 \end{pmatrix} = (1 \ 1 \ 1) \begin{pmatrix} 1 \\ -1 \\ 0 \end{pmatrix} = 0$$

$$d_1^T A d_2 = (1 \ 0 \ -1) \begin{pmatrix} 1 & 1 & 1 \\ 0 & 1 & 1 \\ 0 & 0 & 1 \end{pmatrix} \begin{pmatrix} 1 \\ -1 \\ 0 \end{pmatrix} = (1 \ 1 \ 0) \begin{pmatrix} 1 \\ -1 \\ 0 \end{pmatrix} = 0$$

Thus, d_0, d_1, d_2 are A -conjugate

$$(b) \quad f(x) = \frac{1}{2} x^T A x - b^T x, \quad A = \begin{pmatrix} 1 & 1 & 1 \\ 0 & 1 & 1 \\ 0 & 0 & 1 \end{pmatrix}, \quad b = \begin{pmatrix} 1 \\ 1 \\ 0 \end{pmatrix}, \quad x^0 = \begin{pmatrix} 0 \\ 0 \\ 0 \end{pmatrix}$$

$$x^{k+1} = x^k + \alpha_k d_k \quad \text{with } \alpha_k = -\frac{g_k^T d_k}{d_k^T A d_k} \quad \text{where } g_k = Ax^k - b$$

$$g_0 = Ax^0 - b = \begin{pmatrix} 1 & 1 & 1 \\ 0 & 1 & 1 \\ 0 & 0 & 1 \end{pmatrix} \begin{pmatrix} 0 \\ 0 \\ 0 \end{pmatrix} - \begin{pmatrix} 1 \\ 1 \\ 0 \end{pmatrix} = \begin{pmatrix} -1 \\ -1 \\ 0 \end{pmatrix}$$

$$\alpha_0 = -\frac{g_0^T d_0}{d_0^T A d_0} = -\frac{(1 \ -1 \ 0) \begin{pmatrix} 1 \\ 0 \\ 0 \end{pmatrix}}{(1 \ 0 \ 0) \begin{pmatrix} 1 & 1 & 1 \\ 0 & 1 & 1 \\ 0 & 0 & 1 \end{pmatrix} \begin{pmatrix} 1 \\ 0 \\ 0 \end{pmatrix}} = -\frac{-1}{1} = 1$$

$$x^1 = x^0 + \alpha_0 d_0 = \begin{pmatrix} 0 \\ 0 \\ 0 \end{pmatrix} + 1 \begin{pmatrix} 1 \\ 0 \\ 0 \end{pmatrix} = \begin{pmatrix} 1 \\ 0 \\ 0 \end{pmatrix}$$

$$g_1 = Ax^1 - b = \begin{pmatrix} 1 & 1 & 1 \\ 0 & 1 & 1 \\ 0 & 0 & 1 \end{pmatrix} \begin{pmatrix} 1 \\ 0 \\ 0 \end{pmatrix} - \begin{pmatrix} 1 \\ 1 \\ 0 \end{pmatrix} = \begin{pmatrix} 0 \\ 0 \\ 0 \end{pmatrix} - \begin{pmatrix} 1 \\ 1 \\ 0 \end{pmatrix} = \begin{pmatrix} -1 \\ -1 \\ 0 \end{pmatrix}$$

$$\alpha_1 = -\frac{g_1^T d_1}{d_1^T A d_1} = -\frac{(0 \ -1 \ 0) \begin{pmatrix} 1 \\ 0 \\ -1 \end{pmatrix}}{(1 \ 0 \ -1) \begin{pmatrix} 1 & 1 & 1 \\ 0 & 1 & 1 \\ 0 & 0 & 1 \end{pmatrix} \begin{pmatrix} 1 \\ 0 \\ -1 \end{pmatrix}} = 0$$

$$x^2 = x^1 + \alpha_1 d_1 = \begin{pmatrix} 1 \\ 0 \\ 0 \end{pmatrix} + 0 \cdot \begin{pmatrix} 1 \\ 0 \\ -1 \end{pmatrix} = \begin{pmatrix} 1 \\ 0 \\ 0 \end{pmatrix}$$

$$g_2 = Ax^2 - b = \begin{pmatrix} 1 & 1 & 1 \\ 0 & 1 & 1 \\ 0 & 0 & 1 \end{pmatrix} \begin{pmatrix} 1 \\ 0 \\ 0 \end{pmatrix} - \begin{pmatrix} 1 \\ 1 \\ 0 \end{pmatrix} = \begin{pmatrix} 0 \\ 0 \\ 0 \end{pmatrix} - \begin{pmatrix} 1 \\ 1 \\ 0 \end{pmatrix} = \begin{pmatrix} -1 \\ -1 \\ 0 \end{pmatrix}$$

$$\alpha_2 = -\frac{g_2^T d_2}{d_2^T A d_2} = -\frac{(0 \ -1 \ 0) \begin{pmatrix} 1 \\ -1 \\ 0 \end{pmatrix}}{(1 \ -1 \ 0) \begin{pmatrix} 1 & 1 & 1 \\ 0 & 1 & 1 \\ 0 & 0 & 1 \end{pmatrix} \begin{pmatrix} 1 \\ -1 \\ 0 \end{pmatrix}} = \frac{-1}{(1 \ 0 \ 0) \begin{pmatrix} 1 \\ -1 \\ 0 \end{pmatrix}} = \frac{-1}{1} = -1$$

$$x^3 = x^2 + \alpha_2 d_2 = \begin{pmatrix} 1 \\ 0 \\ 0 \end{pmatrix} + (-1) \begin{pmatrix} 1 \\ -1 \\ 0 \end{pmatrix} = \begin{pmatrix} 0 \\ 1 \\ 0 \end{pmatrix}$$